progress on denormalize

lib/falcon/normalization_lemmas.i.dfy
@@ -50,8 +50,10 @@ module normalization_lemmas {
     }
 
     predicate {:opaque} normalized_values(a: seq<uint16>)
+        ensures normalized_values(a) ==> |a| == N.full;
     {
-        forall i | 0 <= i < |a| :: uint16_is_normalized(a[i])
+        && |a| == N.full
+        && (forall i | 0 <= i < |a| :: uint16_is_normalized(a[i]))
     }
 
     function uint16_buff_as_nelems(a: seq<uint16>): (na: seq<nelem>)
@@ -65,7 +67,6 @@ module normalization_lemmas {
     {
         && b16_iter_inv(iter, heap, if address >= 0 then address else iter.cur_ptr())
         && (index >= 0 ==> iter.index == index)
-        && |iter.buff| == N.full
         && normalized_values(iter.buff)
     }
 
@@ -104,5 +105,47 @@ module normalization_lemmas {
             assert d == sa0 + Q;
             assert d == denormalize(uint16_as_nelem(a0));
         }
+    }
+
+    predicate {:opaque} denormalization_inv(nv: seq<uint16>, dnv: seq<uint16>, i: nat)
+        requires normalized_values(nv);
+        requires buff_is_nsized(dnv);
+    {
+        && reveal normalized_values();
+        && i <= N.full
+        && (forall j | 0 <= j < i :: dnv[j] == denormalize(uint16_as_nelem(nv[j])))
+    }
+
+    lemma denormalization_pre_lemma(nv: seq<uint16>, dnv: seq<uint16>)
+        requires normalized_values(nv);
+        requires buff_is_nsized(dnv);
+        ensures denormalization_inv(nv, dnv, 0);
+    {
+        reveal denormalization_inv();
+    }
+
+    lemma denormalization_peri_lemma(buff: seq<uint16>, dnv: seq<uint16>, i: nat, a1: uint32, b: uint32, c: uint32, d: uint32)
+        requires normalized_values(buff);
+        requires buff_is_nsized(dnv);
+        requires denormalization_inv(buff, dnv, i);
+        requires i < |buff|;
+        requires a1 == uint16_sign_ext(buff[i]);
+        requires b == to_uint32(int32_rs(to_int32(a1), 31));
+        requires c == uint32_and(b, Q);
+        requires d == uint32_add(a1, c);
+        ensures uint16_is_normalized(buff[i]);
+        ensures d == denormalize(uint16_as_nelem(buff[i]));
+        ensures buff_is_nsized(dnv[i := d]);
+        ensures denormalization_inv(buff, dnv[i := d], i + 1);
+    {
+        reveal denormalization_inv();
+        reveal normalized_values();
+        denormalize_lemma(buff, i, a1, b, c, d);
+        var dnv' := dnv[i := d];
+        forall j | 0 <= j <= i
+            ensures dnv'[j] == denormalize(uint16_as_nelem(buff[j]))
+        {
+        } 
+        reveal buff_is_nsized();
     }
 }
